theories/case_studies/vae/vae_adequacy.v
@@ -1,0 +1,1026 @@
+From iris.proofmode Require Import proofmode.
+From cap_machine Require Import logrel interp_weakening monotone.
+From cap_machine Require Import vae vae_spec.
+From cap_machine Require Import switcher assert logrel.
+From cap_machine Require Import mkregion_helpers.
+From cap_machine Require Import region_invariants_revocation region_invariants_allocation.
+From iris.program_logic Require Import adequacy.
+From iris.base_logic Require Import invariants.
+From cap_machine Require Import compartment_layout switcher_adequacy.
+From cap_machine Require Import disjoint_regions_tactics.
+From cap_machine Require Import interp_switcher_call interp_switcher_return.
+
+Class memory_layout `{MP: MachineParameters} := {
+
+    (* switcher *)
+    switcher_layout : @switcherLayout MP;
+    switcher_cmpt : cmptSwitcher;
+
+    (* assert *)
+    assert_cmpt : cmptAssert;
+
+    (* main compartment *)
+    main_cmpt : cmpt ;
+
+    (* adv compartments C *)
+    C_cmpt : cmpt ;
+
+    (* disjointness *)
+    cmpts_disjoints :
+    main_cmpt ## C_cmpt ;
+
+    switcher_cmpt_disjoints :
+    switcher_cmpt_disjoint main_cmpt switcher_cmpt
+    ∧ switcher_cmpt_disjoint C_cmpt switcher_cmpt ;
+
+    assert_cmpt_disjoints :
+    assert_cmpt_disjoint main_cmpt assert_cmpt
+    ∧ assert_cmpt_disjoint C_cmpt assert_cmpt ;
+
+    assert_switcher_disjoints :
+    assert_switcher_disjoint assert_cmpt switcher_cmpt;
+  }.
+
+Definition mk_initial_memory `{memory_layout} (mem: Mem) :=
+  mk_initial_switcher switcher_cmpt ∪
+    mk_initial_assert assert_cmpt ∪
+    mk_initial_cmpt main_cmpt ∪
+    mk_initial_cmpt C_cmpt.
+
+
+Definition is_initial_registers `{memory_layout} (reg: Reg) :=
+  reg !! PC = Some (WCap RX Global (cmpt_b_pcc main_cmpt) (cmpt_e_pcc main_cmpt) (cmpt_a_code main_cmpt)) ∧
+  reg !! cgp = Some (WCap RW Global (cmpt_b_cgp main_cmpt) (cmpt_e_cgp main_cmpt) (cmpt_b_cgp main_cmpt)) ∧
+  reg !! csp = Some (WCap RWL Local (b_stack switcher_cmpt) (e_stack switcher_cmpt) (b_stack switcher_cmpt)) ∧
+  (∀ (r: RegName), r ∉ ({[ PC; cgp; csp ]} : gset RegName) → reg !! r = Some (WInt 0)).
+
+Program Definition is_initial_sregisters `{@memory_layout MP} (sreg : SReg) :=
+  sreg !! MTDC = Some (WCap RWL Local
+                         (@b_trusted_stack MP switcher_layout)
+                         (@e_trusted_stack MP switcher_layout)
+                         (@b_trusted_stack MP switcher_layout)).
+
+Definition is_initial_memory `{@memory_layout MP} (mem: Mem) :=
+  let b_switcher := (@b_switcher MP switcher_layout) in
+  let e_switcher := (@e_switcher MP switcher_layout) in
+  let a_switcher_call := (@a_switcher_call MP switcher_layout) in
+  let ot_switcher := (@ot_switcher MP switcher_layout) in
+  let switcher_entry :=
+    WSentry XSRW_ Local
+      b_switcher
+      e_switcher
+      a_switcher_call
+  in
+  let C_f :=
+    SCap RO Global
+      (cmpt_exp_tbl_pcc C_cmpt)
+      (cmpt_exp_tbl_entries_end C_cmpt)
+      (cmpt_exp_tbl_entries_start C_cmpt)
+  in
+
+  mem = mk_initial_memory mem
+  (* instantiating main *)
+  ∧ (cmpt_imports main_cmpt) =
+  vae_main_imports
+    b_switcher e_switcher a_switcher_call ot_switcher
+    (b_assert assert_cmpt) (e_assert assert_cmpt) C_f
+    (cmpt_exp_tbl_pcc main_cmpt)
+    (cmpt_exp_tbl_entries_end main_cmpt)
+    (cmpt_exp_tbl_entries_start main_cmpt)
+  ∧ (cmpt_code main_cmpt) = (vae_main_code ot_switcher)
+  ∧ (cmpt_data main_cmpt) = vae_main_data
+  ∧ (cmpt_exp_tbl_entries main_cmpt) =
+  (vae_export_table_entries
+      b_switcher e_switcher a_switcher_call ot_switcher
+        (b_assert assert_cmpt) (e_assert assert_cmpt) C_f
+        (cmpt_exp_tbl_pcc main_cmpt)
+        (cmpt_exp_tbl_entries_end main_cmpt)
+        (cmpt_exp_tbl_entries_start main_cmpt)
+    )
+
+  (* instantiating C *)
+  ∧ (cmpt_imports C_cmpt) = [switcher_entry]
+  ∧ Forall is_z (cmpt_code C_cmpt) (* only instructions *)
+  ∧ Forall is_z (cmpt_data C_cmpt) (* TODO generalise: either z or in_region *)
+  ∧ (cmpt_exp_tbl_entries C_cmpt) = [WInt (encode_entry_point 1 1)]
+
+  (* initial stack *)
+  ∧ Forall is_z (stack_content switcher_cmpt)
+.
+
+Lemma mk_initial_cmpt_C_disjoint `{Layout: @memory_layout MP} (m : Mem) :
+  mk_initial_switcher switcher_cmpt ∪ mk_initial_assert assert_cmpt ∪ mk_initial_cmpt main_cmpt
+    ##ₘ mk_initial_cmpt C_cmpt.
+Proof.
+  pose proof cmpts_disjoints as HmainC.
+  pose proof switcher_cmpt_disjoints as (_ & HswitcherC).
+  pose proof assert_cmpt_disjoints as ( _ & HassertC).
+  do 2 rewrite map_disjoint_union_l.
+  repeat split.
+  - symmetry; apply disjoint_switcher_cmpts_mkinitial; done.
+  - symmetry; apply disjoint_assert_cmpts_mkinitial; done.
+  - apply disjoint_cmpts_mkinitial; done.
+Qed.
+
+Lemma mk_initial_cmpt_main_disjoint `{Layout: @memory_layout MP} (m : Mem) :
+  mk_initial_switcher switcher_cmpt ∪ mk_initial_assert assert_cmpt
+    ##ₘ mk_initial_cmpt main_cmpt.
+Proof.
+  pose proof switcher_cmpt_disjoints as (HswitcherMain & _).
+  pose proof assert_cmpt_disjoints as (HassertMain & _).
+  rewrite map_disjoint_union_l.
+  repeat split.
+  - symmetry; apply disjoint_switcher_cmpts_mkinitial; done.
+  - symmetry; apply disjoint_assert_cmpts_mkinitial; done.
+Qed.
+
+Section Adequacy.
+  Context (Σ: gFunctors).
+  Context {cname : CmptNameG}.
+  Context {C : CmptName}.
+  Context {inv_preg: invGpreS Σ}.
+  Context {mem_preg: gen_heapGpreS Addr Word Σ}.
+  Context {reg_preg: gen_heapGpreS RegName Word Σ}.
+  Context {sreg_preg: gen_heapGpreS SRegName Word Σ}.
+  Context {entry_preg : entryGpreS Σ}.
+  Context {seal_store_preg: sealStorePreG Σ}.
+  Context {na_invg: na_invG Σ}.
+  Context {sts_preg: STS_preG Addr region_type Σ}.
+  Context {cstack_preg: CSTACK_preG Σ }.
+  Context {heappreg: heapGpreS Σ}.
+  Context `{MP: MachineParameters}.
+  Context { HCNames : CNames = (list_to_set [C]) }.
+
+  Definition flagN : namespace := nroot .@ "vae" .@ "fail_flag".
+  Definition switcherN : namespace := nroot .@ "vae" .@ "switcher_flag".
+  Definition assertN : namespace := nroot .@ "vae" .@ "assert_flag".
+  Definition vaeN : namespace := nroot .@ "vae" .@ "code".
+
+  Lemma cmdc_adequacy' `{Layout: @memory_layout MP}
+    (reg reg': Reg) (sreg sreg': SReg) (m m': Mem)
+    (es: list cap_lang.expr):
+    is_initial_registers reg →
+    is_initial_sregisters sreg →
+    is_initial_memory m →
+    rtc erased_step ([Seq (Instr Executable)], (reg, sreg, m)) (es, (reg', sreg', m')) →
+    m' !! (flag_assert assert_cmpt) = Some (WInt 0%Z).
+  Proof.
+    intros Hreg Hsreg Hm Hstep.
+    pose proof (@wp_invariance Σ cap_lang _ NotStuck) as WPI. cbn in WPI.
+    pose (fun (c: ExecConf) => c.2 !! (flag_assert assert_cmpt) = Some (WInt 0%Z)) as state_is_good.
+    specialize (WPI (Seq (Instr Executable)) (reg, sreg, m) es (reg', sreg', m')
+                  (state_is_good (reg', sreg', m'))).
+    eapply WPI. 2: assumption. intros Hinv κs. clear WPI.
+
+    set b_switcher := (@b_switcher MP switcher_layout).
+    set e_switcher := (@e_switcher MP switcher_layout).
+    set a_switcher_call := (@a_switcher_call MP switcher_layout).
+    set ot_switcher := (@ot_switcher MP switcher_layout).
+    set a_switcher_return := (@a_switcher_return MP switcher_layout).
+    set b_trusted_stack := (@b_trusted_stack MP switcher_layout).
+    set e_trusted_stack := (@e_trusted_stack MP switcher_layout).
+    set switcher_size := (@switcher_size MP switcher_layout).
+    set switcher_call_entry_point := (@switcher_call_entry_point MP switcher_layout).
+    set switcher_return_entry_point := (@switcher_return_entry_point MP switcher_layout).
+
+    pose proof Hm as Hm'.
+    destruct Hm as (Hm
+                    & main_imports & main_code & main_data & main_exp_tbl
+                    & C_imports & C_code & C_data & C_exp_tbl
+                    & Hstack
+                   ).
+    iMod (gen_heap_init (reg:Reg)) as (reg_heapg) "(Hreg_ctx & Hreg & _)".
+    iMod (gen_heap_init (sreg:SReg)) as (sreg_heapg) "(Hsreg_ctx & Hsreg & _)".
+    iMod (gen_heap_init (m:Mem)) as (mem_heapg) "(Hmem_ctx & Hmem & _)".
+    iMod (seal_store_init ({[ ot_switcher ]} : gset _)) as (seal_storeg) "Hseal_store".
+    set (
+        C_f :=
+       (WCap RO Global (cmpt_exp_tbl_pcc C_cmpt) (cmpt_exp_tbl_entries_end C_cmpt)
+         (cmpt_exp_tbl_entries_start C_cmpt))
+      ).
+    set (awk_f :=
+          (WCap RO Global
+             (cmpt_exp_tbl_pcc main_cmpt) (cmpt_exp_tbl_entries_end main_cmpt)
+             (cmpt_exp_tbl_pcc main_cmpt ^+ 2)%a)
+        ).
+    assert (C_f ≠ awk_f) as Hneq_entries.
+    { intro H ; subst awk_f C_f ; simplify_eq.
+      pose proof cmpts_disjoints as Hdisjoint.
+      rewrite /disjoint /Cmpt_Disjoint /disjoint_cmpt /cmpt_region in Hdisjoint.
+      assert (
+          cmpt_exp_tbl_region main_cmpt  ## cmpt_exp_tbl_region C_cmpt
+        ) as Hdis by set_solver+Hdisjoint.
+      rewrite /cmpt_exp_tbl_region in Hdis.
+      apply stdpp_extra.list_to_set_disj in Hdis.
+      rewrite H H0 in Hdis.
+      assert (
+          list_to_set
+            (finz.seq_between (cmpt_exp_tbl_pcc main_cmpt) (cmpt_exp_tbl_entries_end main_cmpt))
+            ≠ (∅ : gset Addr)
+        ) as Hemp; [|set_solver+Hdis Hemp].
+      pose proof (cmpt_exp_tbl_pcc_size main_cmpt) as Hc.
+      pose proof (cmpt_exp_tbl_cgp_size main_cmpt) as Hc'.
+      pose proof (cmpt_exp_tbl_entries_size main_cmpt) as Hc''.
+      rewrite finz_seq_between_cons ; last (solve_addr+ Hc Hc' Hc'').
+      set_solver+.
+    }
+
+    iMod (
+       entry_init (
+           {[
+               (seal_capability C_f ot_switcher) := 1;
+               (borrow (seal_capability C_f ot_switcher)) := 1;
+               (seal_capability awk_f ot_switcher) := 1;
+               (borrow (seal_capability awk_f ot_switcher)) := 1
+           ]}
+
+         )
+      ) as (entry_g) "Hentries".
+    iDestruct (big_sepM_insert_delete with "Hentries") as "[#Hentry_Cf Hentries]"
+    ; repeat (rewrite delete_insert_ne ; last (subst awk_f C_f ; intro ; simplify_eq; by rewrite H H0 H1 in Hneq_entries)).
+    iDestruct (big_sepM_insert_delete with "Hentries") as "[Hentry_Cf' Hentries]"
+    ; repeat (rewrite delete_insert_ne ; last (subst awk_f C_f ; intro ; simplify_eq; by rewrite H H0 H1 in Hneq_entries)).
+    iDestruct (big_sepM_insert_delete with "Hentries") as "[#Hentry_awkf Hentries]"
+    ; repeat (rewrite delete_insert_ne ; last (subst awk_f C_f ; intro ; simplify_eq; by rewrite H H0 H1 in Hneq_entries)).
+    iDestruct (big_sepM_insert_delete with "Hentries") as "[Hentry_awkf' _]"
+    ; repeat (rewrite delete_insert_ne ; last (subst awk_f C_f ; intro ; simplify_eq; by rewrite H H0 H1 in Hneq_entries)).
+    subst C_f awk_f; cbn.
+    set (C_f := (SCap RO Global (cmpt_exp_tbl_pcc C_cmpt) (cmpt_exp_tbl_entries_end C_cmpt)
+                   (cmpt_exp_tbl_entries_start C_cmpt))).
+    set (C_f' := (SCap RO Local (cmpt_exp_tbl_pcc C_cmpt) (cmpt_exp_tbl_entries_end C_cmpt)
+                   (cmpt_exp_tbl_entries_start C_cmpt))).
+    set (awk_f :=
+          (SCap RO Global (cmpt_exp_tbl_pcc main_cmpt)
+                       (cmpt_exp_tbl_entries_end main_cmpt) (cmpt_exp_tbl_pcc main_cmpt ^+ 2)%a)
+        ).
+    set (awk_f' :=
+          (SCap RO Local (cmpt_exp_tbl_pcc main_cmpt)
+                        (cmpt_exp_tbl_entries_end main_cmpt) (cmpt_exp_tbl_pcc main_cmpt ^+ 2)%a)
+        ).
+
+    unshelve iMod (gen_sts_init 0) as (stsg) "Hsts"; eauto. (*XX*)
+    iMod (gen_cstack_init []) as (cstackg) "[Hcstk_full Hcstk_frag]".
+    iMod (heap_init) as (heapg) "HRELS".
+
+    iDestruct (big_sepS_elements with "Hsts") as "Hsts_C".
+    iDestruct (big_sepS_elements with "HRELS") as "HRELS_C".
+    rewrite HCNames.
+    pose proof (NoDup_singleton C) as HCNoDup.
+    setoid_rewrite elements_list_to_set; auto.
+    rewrite !big_sepL_singleton.
+
+    iMod (@na_alloc Σ na_invg) as (logrel_nais) "Hna".
+
+    pose ceriseg := CeriseG Σ Hinv mem_heapg reg_heapg sreg_heapg entry_g.
+    pose logrel_na_invs := Build_logrel_na_invs _ na_invg logrel_nais.
+    pose switcher_layout_g := (@switcher_layout MP Layout).
+
+    pose proof (
+        @vae_init_spec Σ ceriseg seal_storeg _ _ _ logrel_na_invs _ _  switcher_layout_g C
+      ) as Spec.
+
+    (* Get initial sregister mtdc *)
+    iDestruct (big_sepM_lookup with "Hsreg") as "Hmtdc"; eauto.
+
+    (* Separate all compartments *)
+    rewrite {2}Hm.
+    rewrite /mk_initial_memory.
+    iDestruct (big_sepM_union with "Hmem") as "[Hmem Hcmpt_C]".
+    { eapply mk_initial_cmpt_C_disjoint; eauto. }
+    iDestruct (big_sepM_union with "Hmem") as "[Hmem Hcmpt_main]".
+    { eapply mk_initial_cmpt_main_disjoint; eauto. }
+    iDestruct (big_sepM_union with "Hmem") as "[Hcmpt_switcher Hcmpt_assert]".
+    { pose proof assert_switcher_disjoints; symmetry; eapply disjoint_assert_switcher_mkinitial ; eauto. }
+
+    (* Assert *)
+    rewrite /mk_initial_assert.
+    iDestruct (big_sepM_union with "Hcmpt_assert") as "[Hassert Hassert_flag]".
+    { eapply cmpt_assert_flag_mregion_disjoint ; eauto. }
+    iDestruct (big_sepM_union with "Hassert") as "[Hassert Hassert_cap]".
+    { eapply cmpt_assert_cap_mregion_disjoint ; eauto. }
+    rewrite /cmpt_assert_flag_mregion.
+    rewrite /mkregion.
+    rewrite finz_seq_between_singleton.
+    2: { pose proof (assert_flag_size assert_cmpt) as H; solve_addr+H. }
+    cbn.
+    iDestruct (big_sepM_insert with "Hassert_flag") as "[Hassert_flag _]"; first done.
+    iMod (inv_alloc flagN ⊤ (flag_assert assert_cmpt ↦ₐ WInt 0%Z) with "Hassert_flag")%I
+     as "#Hinv_assert_flag".
+    rewrite /cmpt_assert_cap_mregion.
+    rewrite /mkregion.
+    rewrite finz_seq_between_singleton.
+    2: { pose proof (assert_cap_size assert_cmpt) as H; solve_addr+H. }
+    cbn.
+    iDestruct (big_sepM_insert with "Hassert_cap") as "[Hassert_cap _]"; first done.
+
+    rewrite /cmpt_assert_code_mregion.
+    iDestruct (mkregion_prepare with "[Hassert]") as ">Hassert"; auto.
+    { apply (assert_code_size assert_cmpt). }
+    iAssert (assert.assert_inv
+               (b_assert assert_cmpt)
+               (e_assert assert_cmpt)
+               (flag_assert assert_cmpt))
+            with "[Hassert Hassert_cap]" as "Hassert".
+    { rewrite /assert.assert_inv. iExists (cap_assert assert_cmpt).
+      rewrite /codefrag /region_pointsto.
+      replace (b_assert assert_cmpt ^+ length assert_subroutine_instrs)%a
+        with (cap_assert assert_cmpt).
+      2: { pose proof (assert_code_size assert_cmpt); solve_addr+H. }
+      iFrame.
+      iSplit; first (iPureIntro ; apply (assert_code_size assert_cmpt)).
+      iSplit; iPureIntro.
+      + apply (assert_cap_size assert_cmpt).
+      + by rewrite (assert_flag_size assert_cmpt).
+    }
+    iMod (na_inv_alloc logrel.logrel_nais _ assertN _ with "Hassert") as "#Hassert".
+
+    (* Switcher *)
+    rewrite /mk_initial_switcher.
+    iDestruct (big_sepM_union with "Hcmpt_switcher") as "[Hswitcher Hstack]".
+    { eapply cmpt_switcher_stack_mregion_disjoint ; eauto. }
+    iDestruct (big_sepM_union with "Hswitcher") as "[Hswitcher Htrusted_stack]".
+    { eapply cmpt_switcher_trusted_stack_mregion_disjoint ; eauto. }
+
+    rewrite /cmpt_switcher_code_mregion.
+    iDestruct (big_sepM_union with "Hswitcher") as "[Hswitcher_sealing Hswitcher]".
+    { eapply cmpt_switcher_code_stack_mregion_disjoint ; eauto.
+      exact switcher_cmpt.
+    }
+    iEval (rewrite /mkregion) in "Hswitcher_sealing".
+    rewrite finz_seq_between_singleton.
+    2: { apply switcher_call_entry_point. }
+    iEval (cbn) in "Hswitcher_sealing".
+    iDestruct (big_sepM_insert with "Hswitcher_sealing") as "[Hswitcher_sealing _]"; first done.
+    iDestruct (mkregion_prepare with "[Hswitcher]") as ">Hswitcher"; auto.
+    { apply switcher_size. }
+    rewrite /cmpt_switcher_trusted_stack_mregion.
+    iDestruct (mkregion_prepare with "[Htrusted_stack]") as ">Htrusted_stack"; auto.
+    { apply (trusted_stack_size switcher_cmpt). }
+    rewrite  big_sepS_singleton.
+    iMod (seal_store_update_alloc _ ( ot_switcher_propC ) with "Hseal_store") as "#Hsealed_pred_ot_switcher".
+    iAssert ( switcher_preamble.switcher_inv )
+      with "[Hswitcher Hswitcher_sealing Htrusted_stack Hcstk_full Hmtdc]" as "Hswitcher".
+    {
+      rewrite /switcher_preamble.switcher_inv /codefrag /region_pointsto.
+      replace (a_switcher_call ^+ length switcher_instrs)%a
+        with e_switcher.
+      2: { pose proof switcher_size as H.
+           subst a_switcher_call e_switcher.
+           solve_addr+H.
+      }
+      iFrame "∗#".
+      iExists (tl (trusted_stack_content switcher_cmpt)).
+      iSplitR; first (iPureIntro; apply (ot_switcher_size switcher_cmpt)).
+      pose proof (trusted_stack_content_base_zeroed switcher_cmpt) as Htstk_head.
+      pose proof (trusted_stack_size switcher_cmpt) as Htstk_size.
+      destruct (trusted_stack_content switcher_cmpt); cbn in Htstk_head; simplify_eq.
+      rewrite finz_seq_between_cons; last solve_addr+Htstk_size.
+      iDestruct "Htrusted_stack" as "[Hbase_stack Htrusted_stack]".
+      iFrame.
+      iSplitL; last (iPureIntro ; by rewrite finz_add_0).
+      subst switcher_layout_g.
+      iSplit; iPureIntro; solve_addr.
+    }
+    iMod (na_inv_alloc logrel.logrel_nais _ switcherN _ with "Hswitcher") as "#Hswitcher".
+
+    (* CMPT C *)
+    iEval (rewrite /mk_initial_cmpt) in "Hcmpt_C".
+    iDestruct (big_sepM_union with "Hcmpt_C") as "[HC HC_etbl]".
+    { eapply cmpt_exp_tbl_disjoint ; eauto. }
+    iDestruct (big_sepM_union with "HC") as "[HC_code HC_data]".
+    { eapply cmpt_cgp_disjoint ; eauto. }
+    rewrite /cmpt_pcc_mregion.
+    iDestruct (big_sepM_union with "HC_code") as "[HC_imports HC_code]".
+    { eapply cmpt_code_disjoint ; eauto. }
+    rewrite C_imports.
+    iEval (rewrite /mkregion) in "HC_imports".
+    rewrite (finz_seq_between_singleton (cmpt_b_pcc C_cmpt)).
+    2: { pose proof (cmpt_import_size C_cmpt) as HC_import_size.
+         by rewrite C_imports /= in HC_import_size.
+    }
+    iDestruct (big_sepM_insert with "HC_imports") as "[HC_imports _]"; first done.
+    rewrite /cmpt_cgp_mregion.
+    iDestruct (mkregion_prepare with "[HC_code]") as ">HC_code"; auto.
+    { apply (cmpt_code_size C_cmpt). }
+    iDestruct (mkregion_prepare with "[HC_data]") as ">HC_data"; auto.
+    { apply (cmpt_data_size C_cmpt). }
+
+    (* Initialises the world for C *)
+    cbn.
+    iAssert (region (∅, (∅, ∅)) C) with "[HRELS_C]" as "Hr_C".
+    { rewrite region_eq /region_def. iExists ∅, ∅. iFrame.
+      rewrite /= !dom_empty_L //. repeat iSplit; eauto.
+      rewrite /region_map_def. by rewrite big_sepM_empty. }
+
+    iMod (extend_region_perm_sepL2 _ (∅, (∅, ∅)) C
+            (finz.seq_between (cmpt_a_code C_cmpt) (cmpt_e_pcc C_cmpt))
+            (cmpt_code C_cmpt)
+            RX interpC
+           with "Hsts_C Hr_C [HC_code]") as "(Hr_C & #HC_code & Hsts_C)".
+    { done. }
+    { apply Forall_true. intros.
+      by rewrite lookup_empty.
+    }
+    {
+      iApply (big_sepL2_mono ((fun (_ : nat) (k : finz.finz MemNum) (v : Word) =>
+                                 pointsto k (DfracOwn (pos_to_Qp 1)) v)) with "[HC_code]").
+      - intros k v1 v2 Hv1 Hv2. cbn. iIntros; iFrame.
+        pose proof (Forall_lookup_1 _ _ _ _ C_code Hv2) as Hncap.
+        destruct v2; [| by inversion Hncap..].
+        rewrite /interpC /safeC fixpoint_interp1_eq /=.
+        iSplit; eauto.
+        iApply future_priv_mono_interp_z.
+      - iFrame.
+    }
+    iMod (extend_region_perm_sepL2 _ _ C
+            (finz.seq_between (cmpt_b_cgp C_cmpt) (cmpt_e_cgp C_cmpt))
+            (cmpt_data C_cmpt)
+            RW interpC
+           with "Hsts_C Hr_C [HC_data]") as "(Hr_C & #HC_data & Hsts_C)".
+    { done. }
+    { apply Forall_forall. intros a Ha.
+      rewrite std_sta_update_multiple_lookup_same_i; auto.
+      pose proof (cmpt_cgp_disjoint C_cmpt) as Hdisjoint.
+      apply map_disjoint_dom_1 in Hdisjoint.
+      rewrite /cmpt_pcc_mregion dom_union_L in Hdisjoint.
+      rewrite disjoint_union_l in Hdisjoint.
+      destruct Hdisjoint as [_ Hdisjoint].
+      pose proof (cmpt_data_size C_cmpt) as Hsize_data.
+      pose proof (cmpt_code_size C_cmpt) as Hsize_code.
+      rewrite !dom_mkregion_eq in Hdisjoint; auto.
+      apply list_to_set_disj_2 in Hdisjoint.
+      rewrite /disjoint /set_disjoint_instance in Hdisjoint.
+      intro Ha'.
+      apply (Hdisjoint a); auto.
+    }
+    {
+      iApply (big_sepL2_mono ((fun (_ : nat) (k : finz.finz MemNum) (v : Word) =>
+                                 pointsto k (DfracOwn (pos_to_Qp 1)) v)) with "HC_data").
+      intros k v1 v2 Hv1 Hv2. cbn. iIntros; iFrame.
+      pose proof (Forall_lookup_1 _ _ _ _ C_data Hv2) as Hncap.
+      destruct v2; [| by inversion Hncap..].
+      rewrite /interpC /safeC fixpoint_interp1_eq /=.
+      iSplit; eauto.
+      iApply future_priv_mono_interp_z.
+    }
+
+    iMod (extend_region_perm_sepL2 _ _ C
+            [cmpt_b_pcc C_cmpt]
+            (cmpt_imports C_cmpt)
+            RX interpC
+           with "Hsts_C Hr_C [HC_imports]") as "(Hr_C & [#HC_imports _] & Hsts_C)".
+    { done. }
+    { apply Forall_forall.
+      intros a Ha.
+      apply elem_of_list_singleton in Ha; simplify_eq.
+      rewrite std_sta_update_multiple_lookup_same_i; auto.
+      + rewrite std_sta_update_multiple_lookup_same_i; auto.
+        pose proof (cmpt_import_size C_cmpt) as HC.
+        apply not_elem_of_finz_seq_between.
+        rewrite C_imports in HC.
+        left; solve_addr+HC.
+      + pose proof (cmpt_disjointness C_cmpt) as HC.
+        apply disjoint_regions_tactics.disjoint_list_cons in HC
+        ; destruct HC as [HC _].
+        rewrite union_list_cons in HC.
+        cbn in HC.
+        assert (
+            finz.seq_between (cmpt_b_pcc C_cmpt) (cmpt_e_pcc C_cmpt)
+              ## finz.seq_between (cmpt_b_cgp C_cmpt) (cmpt_e_cgp C_cmpt)
+          ) as HC' by set_solver+HC
+        ; clear HC.
+        intro Hcontra ; eapply HC'; eauto.
+        pose proof (cmpt_import_size C_cmpt) as H.
+        rewrite C_imports /= in H.
+        pose proof (cmpt_code_size C_cmpt) as H'.
+        apply elem_of_finz_seq_between; solve_addr+H H'.
+    }
+    {
+      rewrite C_imports; cbn; iFrame.
+      rewrite /interpC /safeC /=.
+      iSplit; first iApply interp_switcher_call; eauto.
+      (* TODO make lemma *)
+      iModIntro.
+      iIntros (???) "?"; iApply interp_switcher_call; eauto.
+    }
+
+    iDestruct (mkregion_prepare with "[Hstack]") as ">Hstack"; auto.
+    { apply (stack_size switcher_cmpt). }
+    iMod ( extend_region_temp_sepL2 _ _ _
+             (finz.seq_between (b_stack switcher_cmpt) (e_stack switcher_cmpt))
+             (stack_content switcher_cmpt)
+             RWL interpC
+           with "Hsts_C Hr_C [Hstack]")
+           as "(Hr_C & #Hrel_stk_C & Hsts_C)".
+    { done. }
+    { apply Forall_forall; intros a Ha; cbn.
+      pose proof (cmpt_import_size C_cmpt) as H.
+      rewrite C_imports /= in H.
+      pose proof (cmpt_code_size C_cmpt) as H'.
+      pose proof switcher_cmpt_disjoints as (_ & Hc).
+
+      rewrite lookup_insert_ne.
+      2: { intro Hcontra.
+           assert (a ∈ finz.seq_between (cmpt_b_pcc C_cmpt) (cmpt_e_pcc C_cmpt)).
+           { rewrite -Hcontra.
+             apply elem_of_finz_seq_between; solve_addr+H H'.
+           }
+           apply (Hc a).
+           + rewrite /cmpt_switcher_region.
+             eapply elem_of_union;eauto.
+           + eapply elem_of_union;eauto.
+             left; eapply elem_of_union;eauto.
+      }
+      rewrite std_sta_update_multiple_lookup_same_i.
+      2: { intro Hcontra.
+           apply (Hc a); eauto.
+           + eapply elem_of_union;eauto.
+           + eapply elem_of_union;eauto.
+             left;eapply elem_of_union;eauto.
+      }
+      rewrite std_sta_update_multiple_lookup_same_i; first done.
+      intro Hcontra.
+      apply (Hc a); eauto.
+      + eapply elem_of_union;eauto.
+      + eapply elem_of_union;eauto.
+        left;eapply elem_of_union;eauto.
+        left.
+        rewrite elem_of_finz_seq_between in Hcontra.
+        apply elem_of_finz_seq_between; solve_addr+H H' Hcontra.
+    }
+    {
+      iApply (big_sepL2_mono ((fun (_ : nat) (k : finz.finz MemNum) (v : Word) =>
+                                 pointsto k (DfracOwn (pos_to_Qp 1)) v)) with "Hstack").
+      intros k v1 v2 Hv1 Hv2. cbn. iIntros; iFrame.
+      pose proof (Forall_lookup_1 _ _ _ _ Hstack Hv2) as Hncap.
+      destruct v2; [| by inversion Hncap..].
+      rewrite /interpC /safeC fixpoint_interp1_eq /=.
+      iSplit; eauto.
+      iApply future_pub_mono_interp_z.
+    }
+
+    match goal with
+    | H: _ |- context [  (sts_full_world ?W C) ] => set (Winit_C := W)
+    end.
+
+
+    iEval (rewrite /cmpt_exp_tbl_mregion) in "HC_etbl".
+    iDestruct (big_sepM_union with "HC_etbl") as "[HC_etbl HC_etbl_entries]".
+    { eapply cmpt_exp_tbl_entries_disjoint. }
+    iDestruct (big_sepM_union with "HC_etbl") as "[HC_etbl_pcc HC_etbl_cgp]".
+    { eapply cmpt_exp_tbl_pcc_cgp_disjoint. }
+    iDestruct (mkregion_prepare with "[HC_etbl_entries]") as ">HC_etbl_entries"; auto.
+    { apply cmpt_exp_tbl_entries_size. }
+    iDestruct (mkregion_prepare with "[HC_etbl_pcc]") as ">HC_etbl_pcc"; auto.
+    { cbn; apply cmpt_exp_tbl_pcc_size. }
+    iDestruct (mkregion_prepare with "[HC_etbl_cgp]") as ">HC_etbl_cgp"; auto.
+    { cbn; apply cmpt_exp_tbl_cgp_size. }
+    iEval (rewrite C_exp_tbl) in "HC_etbl_entries".
+    rewrite (finz_seq_between_singleton (cmpt_exp_tbl_entries_start C_cmpt)).
+    2: {
+      pose proof (cmpt_exp_tbl_entries_size C_cmpt) as H1.
+      by rewrite C_exp_tbl in H1; cbn in H1.
+    }
+    rewrite (finz_seq_between_singleton (cmpt_exp_tbl_pcc C_cmpt))
+    ; last (apply cmpt_exp_tbl_pcc_size).
+    rewrite (finz_seq_between_singleton (cmpt_exp_tbl_cgp C_cmpt))
+    ; last (apply cmpt_exp_tbl_cgp_size).
+    rewrite !big_sepL2_singleton.
+
+    iMod (inv_alloc (switcher_preamble.export_table_PCCN (nroot .@ C)) ⊤ _
+           with "HC_etbl_pcc")%I as "#HC_etbl_pcc".
+    iMod (inv_alloc (switcher_preamble.export_table_CGPN (nroot .@ C)) ⊤ _
+           with "HC_etbl_cgp")%I as "#HC_etbl_cgp".
+    iMod (inv_alloc (switcher_preamble.export_table_entryN (nroot .@ C) (cmpt_exp_tbl_entries_start C_cmpt)) ⊤ _
+           with "HC_etbl_entries")%I as "#HC_etbl_entries".
+
+    iAssert (interp Winit_C C
+               (WCap RX Global (cmpt_b_pcc C_cmpt) (cmpt_e_pcc C_cmpt) (cmpt_b_pcc C_cmpt)%a)
+            )%I as "#Hinterp_pcc_C".
+    { iEval (rewrite fixpoint_interp1_eq /=).
+      iApply big_sepL_intro; iModIntro.
+      iIntros (k a Ha).
+      rewrite finz_seq_between_cons in Ha.
+      2: {
+        pose proof (cmpt_import_size C_cmpt) as H1.
+        pose proof (cmpt_code_size C_cmpt) as H2.
+        rewrite C_imports /= in H1.
+        solve_addr.
+      }
+      pose proof (cmpt_import_size C_cmpt) as Himport_C.
+      rewrite C_imports /= in Himport_C.
+      replace (cmpt_b_pcc C_cmpt ^+ 1)%a with
+        (cmpt_a_code C_cmpt) in Ha by solve_addr+Himport_C.
+      iExists RX, interp.
+      iEval (cbn).
+      iSplit; first done.
+      iSplit; first (iPureIntro ; by apply persistent_cond_interp).
+      iSplit.
+      { destruct k; cbn in Ha ; simplify_eq; first iFrame "HC_imports".
+        rewrite (big_sepL_lookup _ _ _ a); eauto.
+      }
+      iSplit; first (iNext ; by iApply zcond_interp).
+      iSplit; first (iNext ; by iApply rcond_interp).
+      iSplit; first done.
+      assert ((std Winit_C) !! a = Some Permanent).
+      {
+        subst Winit_C.
+        apply elem_of_list_lookup_2 in Ha.
+        rewrite std_sta_update_multiple_lookup_same_i; cycle 1.
+        { pose proof switcher_cmpt_disjoints as ( _ & Hdis_switcher_cmptC).
+          rewrite /switcher_cmpt_disjoint /cmpt_switcher_region /cmpt_region in Hdis_switcher_cmptC.
+          assert
+            (cmpt_switcher_stack_region switcher_cmpt ## cmpt_pcc_region C_cmpt)
+              as Hdis
+              by (set_solver+Hdis_switcher_cmptC).
+          rewrite /cmpt_pcc_region /cmpt_switcher_stack_region in Hdis.
+          intro Hcontra.
+          replace (cmpt_a_code C_cmpt) with (cmpt_b_pcc C_cmpt ^+ 1)%a in Ha by solve_addr+Himport_C.
+          rewrite -(finz_seq_between_cons) in Ha.
+          + apply (Hdis a); auto.
+          + pose proof (cmpt_import_size C_cmpt) as H1.
+            pose proof (cmpt_code_size C_cmpt) as H2.
+            rewrite C_imports /= in H1.
+            solve_addr.
+        }
+        rewrite elem_of_cons in Ha.
+        destruct Ha as [ Ha | Ha ]; simplify_eq.
+        + rewrite std_sta_update_multiple_lookup_in_i; auto; set_solver+.
+        + rewrite std_sta_update_multiple_lookup_same_i; cycle 1.
+          { intro Hcontra. apply elem_of_list_singleton in Hcontra as ->.
+            apply elem_of_finz_seq_between in Ha.
+            solve_addr+Himport_C Ha.
+          }
+          rewrite std_sta_update_multiple_lookup_same_i; cycle 1.
+          { intro Hcontra.
+            assert (
+                (finz.seq_between (cmpt_a_code C_cmpt) (cmpt_e_pcc C_cmpt))
+                  ##
+                  (finz.seq_between (cmpt_b_cgp C_cmpt) (cmpt_e_cgp C_cmpt))
+              ) as Hdis; last set_solver+Ha Hcontra Hdis.
+              clear.
+              pose proof (cmpt_cgp_disjoint C_cmpt) as Hdis.
+              rewrite /cmpt_pcc_mregion /cmpt_cgp_mregion in Hdis.
+              rewrite -/(cmpt_pcc_mregion C_cmpt) -/(cmpt_cgp_mregion C_cmpt) in Hdis.
+              rewrite map_disjoint_dom in Hdis.
+              rewrite dom_cmpt_pcc_mregion dom_cmpt_cgp_mregion /cmpt_pcc_region /cmpt_cgp_region in Hdis.
+              rewrite -list_to_set_disj in Hdis.
+              assert (
+                  finz.seq_between (cmpt_a_code C_cmpt) (cmpt_e_pcc C_cmpt) ⊆ finz.seq_between (cmpt_b_pcc C_cmpt) (cmpt_e_pcc C_cmpt)
+                ); last set_solver.
+              intros a Ha.
+              rewrite !elem_of_finz_seq_between in Ha |- *.
+              pose proof (cmpt_import_size C_cmpt).
+              solve_addr.
+          }
+          rewrite std_sta_update_multiple_lookup_in_i; auto; set_solver+.
+      }
+      iSplit; last done.
+      iApply (monoReq_interp _ _ _ _ Permanent); done.
+    }
+
+    iAssert (interp Winit_C C
+               (WCap RW Global (cmpt_b_cgp C_cmpt) (cmpt_e_cgp C_cmpt) (cmpt_b_cgp C_cmpt)%a)
+            )%I as "#Hinterp_cgp_C".
+    { iEval (rewrite fixpoint_interp1_eq /=).
+      iApply big_sepL_intro; iModIntro.
+      iIntros (k a Ha).
+      iExists RW, interp.
+      iEval (cbn).
+      iSplit; first done.
+      iSplit; first (iPureIntro ; by apply persistent_cond_interp).
+      rewrite (big_sepL_lookup _ (finz.seq_between (cmpt_b_cgp C_cmpt) (cmpt_e_cgp C_cmpt))
+                 k a); eauto.
+      iFrame "HC_data".
+      iSplit; first (iNext ; by iApply zcond_interp).
+      iSplit; first (iNext ; by iApply rcond_interp).
+      iSplit; first (iNext ; by iApply wcond_interp).
+      assert ((std Winit_C) !! a = Some Permanent).
+     { subst Winit_C.
+        apply elem_of_list_lookup_2 in Ha.
+        assert (a ∉ finz.seq_between (b_stack switcher_cmpt) (e_stack switcher_cmpt)).
+        { intro Hcontra.
+          clear -Ha Hcontra.
+          pose proof switcher_cmpt_disjoints as (_&Hdis).
+          set_solver.
+        }
+        assert (a ∉ [cmpt_b_pcc C_cmpt]).
+        { intro Hcontra.
+          clear -Ha Hcontra C_imports.
+          pose proof (cmpt_disjointness C_cmpt) as Hdis.
+          apply disjoint_list_cons in Hdis as [Hdis _].
+          rewrite union_list_cons disjoint_union_r in Hdis.
+          destruct Hdis as [Hdis _].
+          rewrite elem_of_list_singleton in Hcontra; simplify_eq.
+          assert ( cmpt_b_pcc C_cmpt ∈ finz.seq_between (cmpt_b_pcc C_cmpt) (cmpt_e_pcc C_cmpt))
+          ; last set_solver.
+          apply elem_of_finz_seq_between.
+          pose proof (cmpt_import_size C_cmpt) as Hsize; rewrite C_imports in Hsize.
+          pose proof (cmpt_code_size C_cmpt).
+          solve_addr.
+        }
+        repeat (rewrite std_sta_update_multiple_lookup_same_i; last done).
+        rewrite std_sta_update_multiple_lookup_in_i; auto.
+      }
+      iSplit; last done.
+      iApply (monoReq_interp _ _ _ _ Permanent); done.
+    }
+
+    iAssert (interp Winit_C C
+               (WCap RWL Local (b_stack switcher_cmpt) (e_stack switcher_cmpt) (b_stack switcher_cmpt))
+            )%I as "#Hinterp_stack_C".
+    { iEval (rewrite fixpoint_interp1_eq /=).
+      iApply big_sepL_intro; iModIntro.
+      iIntros (k a Ha).
+      iExists RWL, interp.
+      iEval (cbn).
+      iSplit; first done.
+      iSplit; first (iPureIntro ; by apply persistent_cond_interp).
+      rewrite (big_sepL_lookup _ (finz.seq_between (b_stack switcher_cmpt) (e_stack switcher_cmpt))
+                 k a); eauto.
+      iFrame "Hrel_stk_C".
+      iSplit; first (iNext ; by iApply zcond_interp).
+      iSplit; first (iNext ; by iApply rcond_interp).
+      iSplit; first (iNext ; by iApply wcond_interp).
+      assert ((std Winit_C) !! a = Some Temporary).
+      { subst Winit_C.
+        apply elem_of_list_lookup_2 in Ha.
+        rewrite std_sta_update_multiple_lookup_in_i; auto.
+      }
+      iSplit; last done.
+      iApply (monoReq_interp _ _ _ _ Temporary); done.
+    }
+
+    iAssert ( interp Winit_C C (WSealed ot_switcher C_f)) with
+      "[HC_code Hr_C HC_data Hsts_C Hentry_Cf']" as "#Hinterp_C".
+    { iApply (ot_switcher_interp_entry _ _ _ _ 1 1
+               with "[$] [$] [$] [$] [$] [$] [$] [$]"); eauto; last lia.
+      pose proof (cmpt_exp_tbl_entries_size C_cmpt) as H1.
+      pose proof (cmpt_exp_tbl_entries_size C_cmpt) as H2.
+      rewrite C_exp_tbl in H2.
+      solve_addr+H1 H2.
+    }
+    iClear "HC_etbl_pcc HC_etbl_cgp HC_etbl_entries HC_code HC_data Hinterp_pcc_C Hinterp_cgp_C".
+
+    (* CMPT MAIN *)
+    iEval (rewrite /mk_initial_cmpt) in "Hcmpt_main".
+    iDestruct (big_sepM_union with "Hcmpt_main") as "[Hmain Hmain_etbl]".
+    { eapply cmpt_exp_tbl_disjoint ; eauto. }
+    iDestruct (big_sepM_union with "Hmain") as "[Hmain_code Hmain_data]".
+    { eapply cmpt_cgp_disjoint ; eauto. }
+    rewrite /cmpt_pcc_mregion.
+    iDestruct (big_sepM_union with "Hmain_code") as "[Hmain_imports Hmain_code]".
+    { eapply cmpt_code_disjoint ; eauto. }
+    rewrite /cmpt_cgp_mregion.
+    rewrite /cmpt_exp_tbl_mregion.
+    iDestruct (big_sepM_union with "Hmain_etbl") as "[Hmain_etbl Hmain_etbl_entries]".
+    { eapply cmpt_exp_tbl_entries_disjoint ; eauto. }
+    iDestruct (big_sepM_union with "Hmain_etbl") as "[Hmain_etbl_PCC Hmain_etbl_CGP]".
+    { eapply cmpt_exp_tbl_pcc_cgp_disjoint ; eauto. }
+    iDestruct (mkregion_prepare with "[Hmain_imports]") as ">Hmain_imports"; auto.
+    { apply (cmpt_import_size main_cmpt). }
+    iDestruct (mkregion_prepare with "[Hmain_code]") as ">Hmain_code"; auto.
+    { apply (cmpt_code_size main_cmpt). }
+    iDestruct (mkregion_prepare with "[Hmain_data]") as ">Hmain_data"; auto.
+    { apply (cmpt_data_size main_cmpt). }
+    iDestruct (mkregion_prepare with "[Hmain_etbl_PCC]") as ">Hmain_etbl_PCC"; auto.
+    { apply (cmpt_exp_tbl_pcc_size main_cmpt). }
+    iDestruct (mkregion_prepare with "[Hmain_etbl_CGP]") as ">Hmain_etbl_CGP"; auto.
+    { apply (cmpt_exp_tbl_cgp_size main_cmpt). }
+    iDestruct (mkregion_prepare with "[Hmain_etbl_entries]") as ">Hmain_etbl_entries"; auto.
+    { apply (cmpt_exp_tbl_entries_size main_cmpt). }
+    iAssert (
+       [[(cmpt_b_pcc main_cmpt),(cmpt_a_code main_cmpt)]]↦ₐ[[cmpt_imports main_cmpt]]
+     )%I with "[Hmain_imports]" as "Hmain_imports"; first done.
+    iAssert (
+       [[(cmpt_b_cgp main_cmpt),(cmpt_e_cgp main_cmpt)]]↦ₐ[[cmpt_data main_cmpt]]
+     )%I with "[Hmain_data]" as "Hmain_data"; first done.
+    iAssert (
+      codefrag (cmpt_a_code main_cmpt) (cmpt_code main_cmpt)
+     )%I with "[Hmain_code]" as "Hmain_code".
+    { rewrite /codefrag.
+      replace (cmpt_a_code main_cmpt ^+ length (cmpt_code main_cmpt))%a
+        with (cmpt_e_pcc main_cmpt).
+      2: { pose proof (cmpt_code_size main_cmpt) as H ; solve_addr+H. }
+      done.
+    }
+    rewrite main_imports main_code main_data.
+    rewrite main_exp_tbl.
+    iAssert (
+       (cmpt_exp_tbl_pcc main_cmpt) ↦ₐ
+         WCap RX Global (cmpt_b_pcc main_cmpt) (cmpt_e_pcc main_cmpt) (cmpt_b_pcc main_cmpt)
+      )%I with "[Hmain_etbl_PCC]" as "Hmain_etbl_PCC".
+    {
+      rewrite (finz_seq_between_singleton (cmpt_exp_tbl_pcc main_cmpt)).
+      2: { apply (cmpt_exp_tbl_pcc_size main_cmpt). }
+      by rewrite big_sepL2_singleton.
+    }
+    iAssert (
+       (cmpt_exp_tbl_cgp main_cmpt) ↦ₐ
+         WCap RW Global (cmpt_b_cgp main_cmpt) (cmpt_e_cgp main_cmpt) (cmpt_b_cgp main_cmpt)
+      )%I with "[Hmain_etbl_CGP]" as "Hmain_etbl_CGP".
+    {
+      rewrite (finz_seq_between_singleton (cmpt_exp_tbl_cgp main_cmpt)).
+      2: { apply (cmpt_exp_tbl_cgp_size main_cmpt). }
+      by rewrite big_sepL2_singleton.
+    }
+    rewrite /vae_export_table_entries.
+    iAssert (
+       (cmpt_exp_tbl_entries_start main_cmpt) ↦ₐ
+         WInt (encode_entry_point 1 (length (cmpt_imports main_cmpt ++ VAE_main_code_init)))
+      )%I with "[Hmain_etbl_entries]" as "Hmain_etbl_entries".
+    {
+      rewrite (finz_seq_between_singleton (cmpt_exp_tbl_entries_start main_cmpt)).
+      2: {
+        pose proof (cmpt_exp_tbl_entries_size main_cmpt) as H.
+        by rewrite main_exp_tbl /= in H.
+      }
+      rewrite main_imports.
+      by rewrite big_sepL2_singleton.
+    }
+
+    (* Extract registers *)
+    destruct Hreg as (HPC & Hcgp & Hcsp & Hreg).
+    iDestruct (big_sepM_delete _ _ PC with "Hreg") as "[HPC Hreg]"; first by simplify_map_eq.
+    iDestruct (big_sepM_delete _ _ cgp with "Hreg") as "[Hcgp Hreg]"; first by simplify_map_eq.
+    iDestruct (big_sepM_delete _ _ csp with "Hreg") as "[Hcsp Hreg]"; first by simplify_map_eq.
+
+    iCombine "Hmain_imports Hmain_code" as "Hmain_code".
+    iMod (na_inv_alloc logrel.logrel_nais _ vaeN _ with "Hmain_code") as "#Hmain_code".
+    iMod (inv_alloc (export_table_PCCN vaeN) ⊤
+            (cmpt_exp_tbl_pcc main_cmpt
+               ↦ₐ WCap RX Global (cmpt_b_pcc main_cmpt) (cmpt_e_pcc main_cmpt)
+               (cmpt_b_pcc main_cmpt)
+         )%I with "Hmain_etbl_PCC")%I
+     as "#Hinv_etbl_PCC".
+    iMod (inv_alloc (export_table_CGPN vaeN) ⊤
+            (cmpt_exp_tbl_cgp main_cmpt
+               ↦ₐ WCap RW Global (cmpt_b_cgp main_cmpt) (cmpt_e_cgp main_cmpt)
+               (cmpt_b_cgp main_cmpt)
+         )%I with "Hmain_etbl_CGP")%I
+     as "#Hinv_etbl_CGP".
+    iMod (inv_alloc (export_table_entryN vaeN (cmpt_exp_tbl_entries_start main_cmpt)) ⊤
+            (cmpt_exp_tbl_entries_start main_cmpt
+               ↦ₐ WInt (encode_entry_point 1 (length (cmpt_imports main_cmpt ++ VAE_main_code_init)))
+         )%I with "Hmain_etbl_entries")%I
+     as "#Hinv_etbl_entry_awkward".
+
+    replace (cmpt_exp_tbl_entries_start main_cmpt) with
+      (cmpt_exp_tbl_pcc main_cmpt ^+ 2)%a.
+    2: { pose proof (cmpt_exp_tbl_pcc_size main_cmpt) as Hsize_pcc.
+         pose proof (cmpt_exp_tbl_cgp_size main_cmpt) as Hsize_cgp.
+         pose proof (cmpt_exp_tbl_entries_size main_cmpt) as Hsize_entries.
+         rewrite main_exp_tbl /= in Hsize_entries.
+         solve_addr+Hsize_pcc Hsize_cgp Hsize_entries.
+    }
+    replace (cmpt_exp_tbl_cgp main_cmpt) with ((cmpt_exp_tbl_pcc main_cmpt) ^+ 1)%a.
+    2: { pose proof (cmpt_exp_tbl_pcc_size main_cmpt) as Hsize_pcc.
+         pose proof (cmpt_exp_tbl_cgp_size main_cmpt) as Hsize_cgp.
+         solve_addr+Hsize_pcc Hsize_cgp.
+    }
+    rewrite main_imports.
+
+    iPoseProof (Spec _ _ _ _ _ _ _ _
+                  _ (cmpt_exp_tbl_entries_end main_cmpt) _ _ _
+                  _ _ [] [] assertN switcherN vaeN
+                 with "[ $Hassert $Hswitcher $Hmain_code
+                         $Hinv_etbl_PCC $Hinv_etbl_CGP $Hinv_etbl_entry_awkward
+                         $Hna
+                         $Hr_C $Hsts_C
+                         $HPC $Hcgp $Hcsp $Hreg
+                         $Hmain_data
+                         $Hinterp_C $Hcstk_frag
+                         $Hentry_Cf $Hentry_awkf $Hentry_awkf'
+                         $Hsealed_pred_ot_switcher
+                        ]") as "Hspec"; eauto.
+    { solve_ndisj. }
+    { solve_ndisj. }
+    { solve_ndisj. }
+    { pose proof (cmpt_exp_tbl_pcc_size main_cmpt) as Hsize_pcc.
+      pose proof (cmpt_exp_tbl_cgp_size main_cmpt) as Hsize_cgp.
+      pose proof (cmpt_exp_tbl_entries_size main_cmpt) as Hsize_entries.
+      rewrite main_exp_tbl /= in Hsize_entries.
+      solve_addr+Hsize_pcc Hsize_cgp Hsize_entries.
+    }
+    { rewrite !dom_delete_L.
+      rewrite regmap_full_dom; first done.
+      intros r.
+      destruct (decide (r = PC)); simplify_eq.
+      { eexists; eapply HPC. }
+      destruct (decide (r = cgp)); simplify_eq.
+      { eexists; eapply Hcgp. }
+      destruct (decide (r = csp)); simplify_eq.
+      { eexists; eapply Hcsp. }
+      eexists (WInt 0).
+      apply Hreg.
+      clear -n n0 n1; set_solver.
+    }
+    { intros r Hdom.
+     rewrite !dom_delete_L in Hdom.
+     destruct (decide (r = PC)); simplify_eq.
+     { set_solver+Hdom. }
+     destruct (decide (r = cgp)); simplify_eq.
+     { set_solver+Hdom. }
+     destruct (decide (r = csp)); simplify_eq.
+     { set_solver+Hdom. }
+     rewrite !lookup_delete_ne //.
+     exists (WInt 0).
+     apply Hreg.
+     clear -n n0 n1; set_solver.
+    }
+    { rewrite /SubBounds.
+      pose proof (cmpt_import_size main_cmpt) as Hmain_imports.
+      pose proof (cmpt_code_size main_cmpt) as Hmain_code.
+      rewrite -main_code.
+      solve_addr+Hmain_imports Hmain_code.
+    }
+    { pose proof (cmpt_data_size main_cmpt) as Hmain_data.
+      by rewrite -main_data.
+    }
+    { pose proof (cmpt_import_size main_cmpt) as Hmain_imports.
+      by rewrite -Hmain_imports main_imports.
+    }
+    { subst Winit_C.
+      intro Hcontra.
+      assert ( (cmpt_b_cgp main_cmpt)%a ∈ finz.seq_between (cmpt_b_cgp main_cmpt) (cmpt_e_cgp main_cmpt)
+             ) as Hb_cgp_in.
+      { pose proof (cmpt_data_size main_cmpt) as H.
+        rewrite elem_of_finz_seq_between.
+        rewrite main_data in H; cbn.
+        solve_addr+H.
+      }
+      apply elem_of_dom_std_multiple_update in Hcontra.
+      clear -Hcontra Hb_cgp_in C_imports.
+      destruct Hcontra as [Hcontra|Hcontra].
+      - pose proof switcher_cmpt_disjoints as (Hdis&_). set_solver.
+      - pose proof cmpts_disjoints as Hdis.
+        apply elem_of_dom_std_multiple_update in Hcontra.
+        destruct Hcontra as [Hcontra|Hcontra].
+        + assert (cmpt_b_pcc C_cmpt ∈ finz.seq_between (cmpt_b_pcc C_cmpt) (cmpt_e_pcc C_cmpt)).
+          { pose proof (cmpt_import_size C_cmpt) as Hsize ; rewrite C_imports in Hsize.
+            pose proof (cmpt_code_size C_cmpt).
+            rewrite elem_of_finz_seq_between; solve_addr.
+          }
+          rewrite elem_of_list_singleton in Hcontra; rewrite {1}Hcontra in Hb_cgp_in.
+          set_solver.
+        + apply elem_of_dom_std_multiple_update in Hcontra.
+          destruct Hcontra as [Hcontra|Hcontra].
+          * set_solver.
+          * apply elem_of_dom_std_multiple_update in Hcontra.
+            destruct Hcontra as [Hcontra|Hcontra].
+            ** assert ((cmpt_b_cgp main_cmpt)%a ∈ finz.seq_between (cmpt_b_pcc C_cmpt) (cmpt_e_pcc C_cmpt))
+               ; last set_solver.
+               rewrite !elem_of_finz_seq_between in Hcontra |- *.
+               pose proof (cmpt_import_size C_cmpt) as Hsize ; rewrite C_imports in Hsize.
+               solve_addr.
+            ** rewrite /= dom_empty_L in Hcontra; set_solver+Hcontra.
+    }
+    { done. }
+
+    iModIntro.
+    iExists (fun σ _ _ => ( ((gen_heap_interp σ.1.1) ∗ (gen_heap_interp σ.1.2)) ∗ (gen_heap_interp σ.2)))%I.
+    iExists (fun _ => True)%I. cbn. iFrame.
+    iSplitL "Hspec".
+    { iApply (wp_mono with "Hspec"); iIntros (?) "?"; done. }
+
+    iIntros "[ [Hreg' Hsreg'] Hmem']". iExists (⊤ ∖ ↑flagN).
+    iInv flagN as ">Hflag" "Hclose".
+    iDestruct (gen_heap_valid with "Hmem' Hflag") as %Hm'_flag.
+    iModIntro. iPureIntro. rewrite /state_is_good //=.
+  Qed.
+End Adequacy.
+
+Inductive CmptNames_vae := | B .
+Local Instance CmptNames_vae_eq_dec : EqDecision CmptNames_vae.
+Proof. intros C C'; destruct C,C'; solve_decision. Qed.
+Local Instance CmptNames_vae_finite : finite.Finite CmptNames_vae.
+Proof.
+  refine {| finite.enum := [B] |}.
+  + apply NoDup_singleton.
+  + intros []; left.
+Defined.
+
+Local Program Instance CmptNames_vae_CmptNameG : CmptNameG :=
+  {| CmptName := CmptNames_vae; |}.
+
+(** END-TO-END THEOREM *)
+Theorem cmdc_adequacy `{Layout: memory_layout}
+  (reg reg': Reg) (sreg sreg': SReg) (m m': Mem)
+  (es: list cap_lang.expr):
+  is_initial_registers reg →
+  is_initial_sregisters sreg →
+  is_initial_memory m →
+  rtc erased_step ([Seq (Instr Executable)], (reg, sreg, m)) (es, (reg', sreg', m')) →
+  m' !! (flag_assert assert_cmpt) = Some (WInt 0%Z).
+Proof.
+  intros ? ? ? ?.
+  set ( cnames := CmptNames_vae_CmptNameG ).
+  set (Σ := #[invΣ
+              ; gen_heapΣ Addr Word; gen_heapΣ RegName Word; gen_heapΣ SRegName Word
+              ; entryPreΣ ; CSTACK_preΣ
+              ; na_invΣ; sealStorePreΣ
+              ; STS_preΣ Addr region_type ; heapPreΣ
+              ; savedPredΣ (((STS_std_states Addr region_type) * (STS_states * STS_rels)) * CmptName * Word)
+      ]).
+  eapply (@cmdc_adequacy' Σ cnames B); eauto; try typeclasses eauto.
+Qed.
